test_lattice2.lean
@@ -1,0 +1,31 @@
+import OrdinalsInductionRecursion.ExtPreOrd
+
+namespace PreOrd
+
+theorem inter_succ_y_subset {x' : PreOrd}
+  (ih : ∀ y, Subset (inter x' y) x') (y : PreOrd) : Subset (inter_succ_y (inter x') y) (succ x') :=
+  match y with
+  | .zero => .zero_subset _
+  | .succ y' => .succ_subset (.mem_succ (ih y'))
+  | .sup g => .sup_subset fun n => inter_succ_y_subset ih (g n)
+
+theorem inter_subset_left (x y : PreOrd) : Subset (inter x y) x :=
+  match x with
+  | .zero => .zero_subset _
+  | .succ x' => inter_succ_y_subset (fun y => inter_subset_left x' y) y
+  | .sup f => .sup_subset fun n => Subset_sup (inter_subset_left (f n) y) n rfl
+
+theorem inter_succ_y_subset_right {x' y : PreOrd}
+  (ih : ∀ y, Subset (inter x' y) y) : Subset (inter_succ_y (inter x') y) y :=
+  match y with
+  | .zero => .zero_subset _
+  | .succ y' => .succ_subset (.mem_succ (ih y'))
+  | .sup g => .sup_subset fun n => Subset_sup (inter_succ_y_subset_right ih) n rfl
+
+theorem inter_subset_right (x y : PreOrd) : Subset (inter x y) y :=
+  match x with
+  | .zero => .zero_subset _
+  | .succ x' => inter_succ_y_subset_right (fun y => inter_subset_right x' y)
+  | .sup f => .sup_subset fun n => inter_subset_right (f n) y
+
+end PreOrd
