test_sUnion.lean
@@ -1,0 +1,38 @@
+import OrdinalsInductionRecursion.ExtPreOrd
+
+namespace PreOrd
+
+mutual
+  theorem mem_subset_proof {a b : PreOrd} (h : Mem a b) : Subset a b :=
+    match b, h with
+    | _, .mem_succ hsub => subset_succ_mono_proof hsub
+    | _, .mem_sup n hmem => Subset_sup (mem_subset_proof hmem) n rfl
+
+  theorem subset_succ_mono_proof {a b : PreOrd} (h : Subset a b) : Subset a (succ b) :=
+    match a, b, h with
+    | _, _, .zero_subset _ => .zero_subset _
+    | _, _, .succ_subset hmem => .succ_subset (.mem_succ (mem_subset_proof hmem))
+    | _, _, .sup_subset hsub => .sup_subset fun n => subset_succ_mono_proof (hsub n)
+end
+
+theorem sUnion_subset_self_proof (x : PreOrd) : Subset (sUnion x) x :=
+  match x with
+  | .zero => .zero_subset _
+  | .succ x' => subset_succ_mono_proof (Subset_refl x')
+  | .sup f => .sup_subset fun n => Subset_sup (sUnion_subset_self_proof (f n)) n rfl
+
+theorem sUnion_mono_mem_proof {x y : PreOrd} (h : Mem x y) : Subset (sUnion x) y :=
+  Subset_trans (sUnion_subset_self_proof x) (mem_subset_proof h)
+
+theorem mem_sUnion_proof {a b : PreOrd} (h : Mem a b) : Subset a (sUnion b) :=
+  match b, h with
+  | _, .mem_succ hsub => hsub
+  | _, .mem_sup n hmem => Subset_sup (mem_sUnion_proof hmem) n rfl
+
+theorem sUnion_mono_subset_proof {x y : PreOrd} (h : Subset x y) : Subset (sUnion x) (sUnion y) :=
+  match x, y, h with
+  | _, _, .zero_subset _ => .zero_subset _
+  | _, _, .succ_subset hmem => mem_sUnion_proof hmem
+  | _, _, .sup_subset hsub => .sup_subset fun n => sUnion_mono_subset_proof (hsub n)
+
+end PreOrd
