test_trans.lean
@@ -1,0 +1,26 @@
+import OrdinalsInductionRecursion.PreOrd
+
+open PreOrd
+
+mutual
+  theorem Subset_trans' {x y z : PreOrd} (h1 : Subset x y) (h2 : Subset y z) : Subset x z :=
+    match x, y, h1 with
+    | _, _, .zero_subset _ => .zero_subset _
+    | _, _, .succ_subset hmem1 => .succ_subset (Mem_Subset_trans' hmem1 h2)
+    | _, _, .sup_subset hsub1 => .sup_subset fun n => Subset_trans' (hsub1 n) h2
+
+  theorem Mem_Subset_trans' {x y z : PreOrd} (h1 : Mem x y) (h2 : Subset y z) : Mem x z :=
+    match y, z, h2 with
+    | _, _, .zero_subset _ => nomatch h1
+    | _, _, .succ_subset hmem2 =>
+      match x, y, h1 with
+      | _, _, .mem_succ hsub1 => Subset_Mem_trans' hsub1 hmem2
+    | _, _, .sup_subset hsub2 =>
+      match x, y, h1 with
+      | _, _, .mem_sup n hmem1 => Mem_Subset_trans' hmem1 (hsub2 n)
+
+  theorem Subset_Mem_trans' {x y z : PreOrd} (h1 : Subset x y) (h2 : Mem y z) : Mem x z :=
+    match y, z, h2 with
+    | _, _, .mem_succ hsub2 => .mem_succ (Subset_trans' h1 hsub2)
+    | _, _, .mem_sup n hmem2 => .mem_sup n (Subset_Mem_trans' h1 hmem2)
+end
